ROM extended with some high-level transitions (up to collision on a given call, and abstract up to bad). Cleaning up examples directory.

examples/Plug_and_Pray.ec
@@ -20,11 +20,11 @@ const bound : int.
 axiom bound_pos : bound > 0.
 
 module type Game = {
-  fun main(x : tin) : tres
+  proc main(x : tin) : tres
 }.
 
 module Guess(G : Game) = {  
-  fun main(x : tin) : (int * tres) = {
+  proc main(x : tin) : (int * tres) = {
     var i : int;
     var o : tres;
     o = G.main(x);
@@ -42,27 +42,28 @@ lemma PBound &m (G <: Game):
            fst res = if k >= 0 && k < bound then k else 0 ].
 proof strict.
   intros phi psi x_arg.
-  bdhoare_deno (_ : (glob G) = (glob G){m} && x_arg = x ==>
-                       phi (glob G) (snd res)
-                    /\ let k = (psi (glob G) (snd res) ) in
-                       fst res = if k >= 0 && k < bound then k else 0) => //.
-  fun.
+  byphoare (_ : (glob G) = (glob G){m} && x_arg = x ==>
+                phi (glob G) (snd res)
+             /\ let k = (psi (glob G) (snd res) ) in
+                  fst res = if k >= 0 && k < bound then k else 0) => //.
+  pose p:= Pr[G.main(x_arg) @ &m: phi (glob G) res].
+  proc.
   seq 1 : (phi (glob G) o)
-          (Pr[ G.main(x_arg) @ &m: phi (glob G) res ])
+          (p)
           (1%r/bound%r)
           (1%r - Pr[ G.main(x_arg) @ &m: phi (glob G) res ])
           0%r
           (true) => //.
     (* probability equality for 'phi (glob G) o' *)
     call (_ :  (glob G) = (glob G){m} && x = x_arg ==> phi (glob G) res) => //.
-    bypr. progress.
-    equiv_deno (_ : (glob G){1} = (glob G){2} && x{1} = x{2}
-                    ==> (phi (glob G) res){1} = (phi (glob G) res){2}) => //.
-      fun true => //.
+    bypr. progress; rewrite /p.
+    byequiv (_ : (glob G){1} = (glob G){2} && x{1} = x{2}
+             ==> (phi (glob G) res){1} = (phi (glob G) res){2}) => //.
+      proc true => //.
       by smt.
     (* probability of sampling such that Guess.i = psi (glob G) o *)
     rnd; skip; progress.
-    cut W: (lambda (x : int),
+    cut W: (fun (x : int),
               phi (glob G){hr} (snd (x, o{hr})) /\
               fst (x, o{hr}) = (if psi (glob G){hr} (snd (x, o{hr})) >= 0 && psi (glob G){hr} (snd (x, o{hr})) < bound
                                then psi (glob G){hr} (snd (x, o{hr}))
@@ -71,17 +72,17 @@ proof strict.
            ((=)  (if psi (glob G){hr} o{hr} >= 0 && psi (glob G){hr} o{hr} < bound
                   then psi (glob G){hr} o{hr}
                   else 0)).
-    by apply fun_ext; rewrite /Fun.(==); smt.
+    by apply fun_ext; rewrite /ExtEq.(==); smt.
     by rewrite W -/(mu_x _ _) Distr.Dinter.mu_x_def_in; smt.
     (* probability that sampling changes '!phi (glob G) o' to 'phi (glob G) o' zero *)
     rnd. skip. progress.
-    cut W:   (lambda (x : int),
+    cut W:   (fun (x : int),
                 phi (glob G){hr} (snd (x, o{hr})) /\
                 fst (x, o{hr}) =
                if psi (glob G){hr} (snd (x, o{hr})) >= 0 &&
                   psi (glob G){hr} (snd (x, o{hr})) < bound
                then  psi (glob G){hr} (snd (x, o{hr})) else 0)
-           = cpFalse.
-    by apply fun_ext; rewrite /Fun.(==); smt.
+           = False.
+    by apply fun_ext; rewrite /ExtEq.(==); smt.
     by rewrite W; smt.
 qed.
