examples/WhileSampling.ec
@@ -6,7 +6,7 @@ axiom lossless : weight sample = 1%r.
 op test : t -> bool.
 
 module Sample = { 
-  fun sample () : t = { 
+  proc sample () : t = { 
     var r : t;
     r = $sample;
     while (test r) {
@@ -16,19 +16,19 @@ module Sample = {
   }
 }.
 
-axiom pr_ntest : 0%r < (mu sample (cpNot test)).
+axiom pr_ntest : 0%r < (mu sample (!test)).
 
 lemma Sample_lossless : islossless Sample.sample.
 proof.
- fun.
+ proc.
  seq 1 : true => //.
   rnd;skip;smt.
- while true (if test r then 1 else 0) 1 (mu sample (cpNot test)) => //;first smt.
+ while true (if test r then 1 else 0) 1 (mu sample (!test)) => //;first smt.
   intros Hrec.
   seq 1 : true => //.
   by rnd;skip;smt.
   by rnd;skip;smt. 
   split;[apply pr_ntest |  intros z].
-  conseq * (_ : true ==> (cpNot test) r);first smt.
+  conseq * (_ : true ==> (!test) r);first smt.
  rnd;skip;progress;apply mu_sub => x //.
-save.
+qed.
