examples/br93.ec
@@ -1,6 +1,6 @@
-require import RandOrcl.
+require import ROM.
 require import Array.
-require import FMap. import OptionGet.
+require import FMap.
 require import FSet.
 require import Int.
 require import Distr.
@@ -41,38 +41,35 @@ axiom finvof : forall(pk : pkey, sk : skey, x : randomness),
 axiom fofinv : forall(pk : pkey, sk : skey, x : randomness),
  in_supp (pk,sk) keypairs => f pk (finv sk x) = x.
 
-axiom keypair_lossless : mu keypairs cpTrue = 1%r.
+axiom keypair_lossless : mu keypairs True = 1%r.
 
 op uniform : plaintext distr = Plaintext.Dword.dword.
 op uniform_rand : randomness distr = Randomness.Dword.dword.
 
-clone RandOrcl as RandOrcl_BR with 
-type from = randomness, 
-type to = plaintext,
-op dsample = uniform,
-op qO = qH,
-op default = Plaintext.zeros.
-
-import RandOrcl_BR.
-import ROM.
-import WRO_Set.
+clone import ROM.SetLog as RandOrcl_BR with 
+  type from  <- randomness, 
+  type to    <- plaintext,
+  op dsample <- fun (x:randomness), uniform,
+  op qH      <- qH.
+import Lazy.
+import Types.
 
 module type Scheme(RO : Oracle) = {
- fun kg() : (pkey * skey)
- fun enc(pk:pkey, m:plaintext): ciphertext 
+ proc kg() : (pkey * skey)
+ proc enc(pk:pkey, m:plaintext): ciphertext 
 }.
 
 module type Adv(ARO : ARO)  = {
- fun a1 (p : pkey) : (plaintext * plaintext) {ARO.o} 
- fun a2 (c : ciphertext) : bool {ARO.o}
+ proc a1 (p : pkey) : (plaintext * plaintext) {ARO.o} 
+ proc a2 (c : ciphertext) : bool {ARO.o}
 }.
 
 
 module CPA(S : Scheme, A_ : Adv) = {
- module ARO = ARO(RO)
+ module ARO = Log(RO)
  module A = A_(ARO)
  module SO = S(RO)
-  fun main(): bool = {
+  proc main(): bool = {
   var pk:pkey;
   var sk:skey;
   var m0, m1 : plaintext;
@@ -97,13 +94,13 @@ module M = {
 }.
 
 module BR(R : Oracle) : Scheme(R) = {
- fun kg():(pkey * skey) = {
+ proc kg():(pkey * skey) = {
   var (pk, sk): pkey * skey;
   (pk,sk) = $keypairs;
   return (pk,sk);
  }
  
- fun enc(pk:pkey, m:plaintext): ciphertext = {
+ proc enc(pk:pkey, m:plaintext): ciphertext = {
   var h : plaintext;
   M.r = $uniform_rand; 
   h  = R.o(M.r);
@@ -115,13 +112,13 @@ module BR(R : Oracle) : Scheme(R) = {
   (* Step 1: replace the hash call by a random value *)
 
 module BR2(R : Oracle) : Scheme(R) = {
- fun kg():(pkey * skey) = {
+ proc kg():(pkey * skey) = {
   var (pk, sk): (pkey * skey);
   (pk,sk) = $keypairs;
   return (pk,sk);
  }
  
- fun enc(pk:pkey, m:plaintext): ciphertext = {
+ proc enc(pk:pkey, m:plaintext): ciphertext = {
   var h : plaintext;
   M.r = $uniform_rand; 
   h = $uniform; 
@@ -134,20 +131,20 @@ lemma eq1_enc :
 ={pk,RO.m} ==>
 !in_dom M.r{2} RO.m{2} => (={res} /\ eq_except RO.m{1} RO.m{2} M.r{2}) ].
 proof.
- fun;inline RO.o.
+ proc;inline RO.o.
  wp;rnd ((^) m{1}) ((^) m{1}).
  wp;rnd;skip;progress => //;first 2 by smt.
  by rewrite Plaintext.xorwA Plaintext.xorwK;smt.
  by rewrite Plaintext.xorwA Plaintext.xorwK;smt.
  by smt.
  by smt.
-save.
+qed.
 
 module CPA2(S : Scheme, A_ : Adv) = {
- module ARO = ARO(RO)
+ module ARO = Log(RO)
  module A = A_(ARO)
  module SO = S(RO)
-  fun main(): bool = {
+  proc main(): bool = {
   var pk:pkey;
   var sk:skey;
   var m0, m1 : plaintext;
@@ -164,61 +161,58 @@ module CPA2(S : Scheme, A_ : Adv) = {
 }.
 
 
-lemma lossless_ARO_init : islossless ARO(RO).init.
-proof. apply RO_lossless_init. qed.
+lemma lossless_ARO_init : islossless Log(RO).init.
+proof. by apply (Log_init_ll RO); apply RO_init_ll. qed.
 
-lemma lossless_ARO_o : islossless ARO(RO).o.
-proof. 
-  apply RO_lossless_o;apply Plaintext.Dword.lossless. 
-qed.
+lemma lossless_ARO_o : islossless Log(RO).o.
+proof. by apply (Log_o_ll RO); apply RO_o_ll; apply Plaintext.Dword.lossless. qed.
 
 section.
 
-declare module A : Adv {M,RO,ARO}.
+declare module A : Adv {M,RO,Log}.
 
 axiom lossless1 : (forall (O <: ARO), islossless O.o =>  islossless A(O).a1).
 axiom lossless2 : (forall (O <: ARO), islossless O.o =>  islossless A(O).a2).
 
 equiv eq1 :  CPA(BR,A).main ~ CPA2(BR2,A).main : 
 (glob A){1} = (glob A){2} ==>
- (!mem M.r ARO.log){2} => ={res}.
+ (!mem M.r Log.qs){2} => ={res}.
 proof.
- fun.
+ proc.
  swap{2} -2.
- call (_ : (mem M.r ARO.log), 
-           (={ARO.log} /\ eq_except RO.m{1} RO.m{2} M.r{2})).
+ call (_ : (mem M.r Log.qs), 
+           (={Log.qs} /\ eq_except RO.m{1} RO.m{2} M.r{2})).
  intros => O Hll;apply (lossless2 O) => //.
- fun;if;[smt|inline RO.o;wp;rnd|];wp;skip;progress => //; first 5 last; last 6 smt.
-  case (x = M.r){2}; first smt.
-  by cut em: forall a, a => !a => false by smt; (* again, this (the whole reasoning) should be lemma-ized *)
-     cut:= em (in_dom x RO.m){2} _ _=> //; smt.
+ proc;inline RO.o;wp;rnd;wp;skip;progress => //; first 5 last; last 6 smt.
+  case ((x = M.r){2}); first smt.
+  by apply (absurd (in_dom x RO.m){2})=> //; smt.
  intros _ _;apply lossless_ARO_o.
- intros &m;fun;if;[inline RO.o;wp;rnd cpTrue|];wp;skip;progress;smt.
+ intros &m; proc; wp; call (RO_o_ll _); auto; smt.
  call eq1_enc.
  rnd.
- call  (_: ={RO.m,ARO.log} /\
- (forall (x : randomness), mem x ARO.log{2} <=> in_dom x RO.m{2})).
-  fun;if;[smt|inline RO.o;wp;rnd|];wp;skip;progress;smt.
+ call  (_: ={RO.m,Log.qs} /\
+ (forall (x : randomness), mem x Log.qs{2} <=> in_dom x RO.m{2})).
+  proc;inline RO.o;wp;rnd;wp;skip;progress;smt.
   inline CPA(BR,A).SO.kg CPA2(BR2,A).SO.kg.
   inline CPA(BR,A).ARO.init CPA2(BR2,A).ARO.init RO.init;wp;rnd;wp;skip.
   progress;by smt.
-save.
+qed.
 
 lemma foo1 : forall (b:bool), mu {0,1} ((=) b) = 1%r / 2%r.
-proof. intros b; apply (Bool.Dbool.mu_x_def b). save. 
+proof. intros b; apply (Bool.Dbool.mu_x_def b). qed. 
 
-lemma foo2 : mu uniform_rand cpTrue = 1%r.
-proof. apply Randomness.Dword.lossless. save.
+lemma foo2 : mu uniform_rand True = 1%r.
+proof. apply Randomness.Dword.lossless. qed.
 
-lemma foo3 : mu uniform cpTrue = 1%r.
-proof. apply Plaintext.Dword.lossless. save.
+lemma foo3 : mu uniform True = 1%r.
+proof. apply Plaintext.Dword.lossless. qed.
 
 lemma prob1_1 : 
  forall &m,Pr[CPA2(BR2,A).main()  @ &m : res] = 1%r / 2%r.
 proof.
  intros &m.
- bdhoare_deno (_ : true ==> res); trivial.
-   fun.
+ byphoare (_ : true ==> res); trivial.
+   proc.
    rnd ((=) b').
    conseq ( _ : ==> true).
     progress;apply foo1.
@@ -226,37 +220,37 @@ proof.
    intros => O Hll;apply (lossless2 O) => //.
 
     apply lossless_ARO_o.   
-   inline CPA2(BR2,A).SO.enc;do 2! (wp;rnd (cpTrue));wp.
+   inline CPA2(BR2,A).SO.enc;do 2! (wp;rnd (True));wp.
    conseq ( _ : ==> true).
      rewrite foo2; rewrite foo3;progress.
    call (_ : true).
    intros => O Hll;apply (lossless1 O) => //.
      apply lossless_ARO_o.  
    inline CPA2(BR2,A).SO.kg.
-   wp;rnd (cpTrue);wp.
+   wp;rnd (True);wp.
    conseq ( _ : ==> true).
      progress;apply keypair_lossless. 
    call lossless_ARO_init;skip;trivial.
-save.
+qed.
 
 lemma prob1_2 : forall &m,
 Pr[CPA(BR,A).main() @ &m: res] <=
-1%r/2%r + Pr[CPA2(BR2,A).main() @ &m : mem M.r ARO.log].
+1%r/2%r + Pr[CPA2(BR2,A).main() @ &m : mem M.r Log.qs].
 proof.
  intros &m.
  rewrite -(prob1_1 &m) //.
  apply (Real.Trans _ 
-             Pr[CPA2(BR2,A).main() @ &m : res \/ mem M.r ARO.log]).
- equiv_deno (eq1 ) => //;progress;smt.
- rewrite Pr mu_or.  smt.
-save.
+             Pr[CPA2(BR2,A).main() @ &m : res \/ mem M.r Log.qs]).
+ byequiv (eq1 ) => //;progress;smt.
+ rewrite Pr [mu_or].  smt.
+qed.
 
 module type Inverter = {
- fun i(pk : pkey, y : randomness) : randomness
+ proc i(pk : pkey, y : randomness) : randomness
 }.
 
 module OW(I :Inverter) ={
- fun main() : bool ={
+ proc main() : bool ={
  var x : randomness;
  var x' : randomness;
  var y : randomness;
@@ -270,9 +264,9 @@ module OW(I :Inverter) ={
 }.
 
 module BR_OW(A_ : Adv) : Inverter = {
- module ARO = ARO(RO)
+ module ARO = Log(RO)
  module A = A_(ARO)
-  fun i(pk : pkey,y : randomness) : randomness ={
+  proc i(pk : pkey,y : randomness) : randomness ={
   var m0 : plaintext;
   var m1 : plaintext;
   var h : plaintext;
@@ -282,7 +276,7 @@ module BR_OW(A_ : Adv) : Inverter = {
   (m0,m1)  = A.a1(pk);
   h = $uniform; 
   b  = A.a2(y || h);
-  x = Option.proj (FMap.Core.find (lambda p0 p1,f pk p0 = y) RO.m);
+  x = oget (FMap.find (fun p0 p1,f pk p0 = y) RO.m);
    return (x);
  }
 }.
@@ -296,64 +290,62 @@ proof.
  rewrite -(finvof pk sk _ _);first smt.
  rewrite -(finvof pk sk _ _);first smt.
  rewrite Heqf;smt.
-save.
+qed.
 
 equiv eq2 : CPA2(BR2,A).main ~ OW(BR_OW(A)).main : 
- (glob A){1} = (glob A){2} ==> (mem M.r{1} ARO.log{1} => res{2}).
+ (glob A){1} = (glob A){2} ==> (mem M.r{1} Log.qs{1} => res{2}).
 proof.
- fun.
+ proc.
  rnd{1}.
  inline  BR_OW(A).i.
  inline CPA2(BR2, A).ARO.init RO.init CPA2(BR2, A).SO.kg 
  BR_OW(A).ARO.init.
  inline CPA2(BR2,A).SO.enc.
  seq 11 9:
- (={pk,sk,RO.m,ARO.log} /\ pk0{2} = pk{2} /\ 
+ (={pk,sk,RO.m,Log.qs} /\ pk0{2} = pk{2} /\ 
   in_supp (pk{2},sk{2}) keypairs /\
-(glob A){1} = (glob A){2}  /\ (forall x, in_dom x RO.m{1} = mem x ARO.log{1}) /\
+(glob A){1} = (glob A){2}  /\ (forall x, in_dom x RO.m{1} = mem x Log.qs{1}) /\
  M.r{1} = x{2} /\ y0{2} = f pk{2} x{2}).
 
- call (_ : ={RO.m,ARO.log} /\ (forall x, in_dom x RO.m{1} = mem x ARO.log{1})).
- fun;if;[smt|inline RO.o;wp;rnd |];wp;skip;progress=> //.
+ call (_ : ={RO.m,Log.qs} /\ (forall x, in_dom x RO.m{1} = mem x Log.qs{1})).
+ proc;inline RO.o;wp;rnd;wp;skip;progress=> //.
    by rewrite /in_dom dom_set !mem_add -/(in_dom _ _) H.
    by rewrite mem_add; rewrite -H; case (x1 = x{2})=> //=;
-      intros=> ->; rewrite rw_eqT.
+      intros=> ->; smt.
  wp;rnd;swap{1} -7;wp.
- call (_: ={RO.m,ARO.log}  /\ (forall x, in_dom x RO.m{1} = mem x ARO.log{1})).
- fun;if;[smt|inline RO.o;wp;rnd |];wp;skip;progress=> //.
+ call (_: ={RO.m,Log.qs}  /\ (forall x, in_dom x RO.m{1} = mem x Log.qs{1})).
+ proc;inline RO.o;wp;rnd;wp;skip;progress=> //.
    by rewrite /in_dom dom_set !mem_add -/(in_dom _ _) H.
    by rewrite mem_add; rewrite -H; case (x1 = x{2})=> //=;
-      intros=> ->; rewrite rw_eqT.
+      intros=> ->; smt.
  do 2! (wp;rnd);skip;progress;smt.
  wp;skip;progress;first smt.
- elim (find_in
-      (lambda (p0:randomness) (p1:to), f pk{2} p0 = f pk{2} x{2})
-      RO.m{2}
-      _); first exists x{2}; split;smt.
- intros x2 Hfind.
- rewrite Hfind.
- elim (find_cor
-      (lambda (p0:randomness) (p1:to), f pk{2} p0 = f pk{2} x{2})
-      RO.m{2}
-      x2 _).
- assumption.
- delta;simplify.
+ cut find_some:= find_in
+                   (fun (p0:randomness) (p1:plaintext), f pk{2} p0 = f pk{2} x{2})
+                   RO.m{2}
+                   _; first exists x{2}; split;smt.
+ cut: exists x', find (fun p0 (p1:plaintext), f pk{2} p0 = f pk{2} x{2}) RO.m{2} = Some x'.
+    by move: find_some; case (find (fun p0 (p1:plaintext), f pk{2} p0 = f pk{2} x{2}) RO.m{2})=> //; smt.
+ elim=> x' find_def.
+ elim (find_cor (fun (p0:randomness) (p1:plaintext), f pk{2} p0 = f pk{2} x{2})
+                   RO.m{2} x'
+                   _); first smt.
+ rewrite find_def /= /oget /=.
  intros Hin_dom Hf.
- rewrite Option.proj_some.
  apply (f_iny _ _ pk{2} sk{2} _ _);smt.
-save.
+qed.
 
 lemma Reduction &m : 
 Pr[CPA(BR,A).main() @ &m : res] <= 1%r / 2%r + Pr[OW(BR_OW(A)).main() @ &m : res].
 proof.
  apply (Real.Trans _  
-               (1%r/2%r + Pr[CPA2(BR2,A).main() @ &m : mem M.r ARO.log])).
+               (1%r/2%r + Pr[CPA2(BR2,A).main() @ &m : mem M.r Log.qs])).
  apply (prob1_2 &m) => //.
- cut H: (Pr[CPA2(BR2,A).main() @ &m : mem M.r ARO.log] <=
+ cut H: (Pr[CPA2(BR2,A).main() @ &m : mem M.r Log.qs] <=
          Pr[OW(BR_OW(A)).main() @ &m : res]).
-   equiv_deno eq2 => //.
+   byequiv eq2 => //.
  by smt.
-save.
+qed.
 
 lemma Conclusion  &m :
 exists (I<:Inverter), Pr[CPA(BR,A).main() @ &m : res] - 1%r / 2%r <= 
@@ -361,7 +353,7 @@ exists (I<:Inverter), Pr[CPA(BR,A).main() @ &m : res] - 1%r / 2%r <=
 proof.
  exists (BR_OW(A)). 
  by cut h := Reduction &m => //;smt.
-save.
+qed.
 
 end section.
 
