examples/hashed_elgamal_generic.ec
@@ -9,150 +9,6 @@ require (*--*) AWord.
 require (*--*) ROM.
 require (*--*) PKE.
 
-(** We extend the basic lazy random oracle with a generic argument
-    replacing a single oracle call in the middle of an experiment
-    with a random sampling. The probability of distinguishing the
-    two is bounded by the probability that another query in the
-    experiment collides with the one we singled out. Ideally, this
-    should be pushed into either the ROM library, or into a
-    ProveIt-specific context.                                       *)
-theory ROM_Call.
-  type from.
-  type to.
-
-  op dsample: from -> to distr.
-  axiom dsampleL x: mu (dsample x) True = 1%r.
-
-  op qH:int.
-  axiom qH_pos: 0 < qH.
-
-  clone import ROM.Lazy as ROM with
-    type from  <- from,
-    type to    <- to,
-    op dsample <- dsample.
-
-  module type Dist(H:Types.ARO) = {
-    proc a1(): from
-    proc a2(x:to): bool
-  }.
-
-  module ARO(O:Types.ARO) = {
-    var qs:from set
-
-    proc o(x:from): to = {
-      var r = witness;
-
-      if (card qs < qH) {
-        r  = O.o(x);
-        qs = add x qs;
-      }
-      return r;
-    }
-  }.
-
-  module Bounder(D:Dist,O:Types.ARO) = {
-    module D' = D(ARO(O))
-
-    proc a1 = D'.a1
-    proc a2 = D'.a2
-  }.
-
-  module G0(D:Dist, H:Types.Oracle) = {
-    module D = Bounder(D,H)
-
-    proc main(): bool = {
-      var x, y, b;
-
-      H.init();
-      ARO.qs = FSet.empty;
-      x = D.a1();
-      y = H.o(x);
-      b = D.a2(y);
-      return b;
-    }
-  }.
-
-  module G1(D:Dist, H:Types.Oracle) = {
-    module D = Bounder(D,H)
-
-    var x:from
-
-    proc main(): bool = {
-      var y, b;
-
-      H.init();
-      ARO.qs = FSet.empty;
-      x = D.a1();
-      y = $dsample x;
-      b = D.a2(y);
-      return b;
-    }
-  }.
-
-  module G2(D:Dist, H:Types.Oracle) = {
-    module D = Bounder(D,H)
-
-    var x:from
-
-    proc main(): bool = {
-      var y, b;
-
-      H.init();
-      ARO.qs = FSet.empty;
-      x = D.a1();
-      y = $dsample x;
-      b = D.a2(y);
-      return mem x ARO.qs;
-    }
-  }.
-
-  lemma Abstract_Bad (D <: Dist {Bounder, RO, G1, G2}) &m:
-    (forall (H <: Types.ARO {D}), islossless H.o => islossless D(H).a1) =>
-    (forall (H <: Types.ARO {D}), islossless H.o => islossless D(H).a2) =>
-    Pr[G0(D,RO).main() @ &m: res]
-    <= Pr[G1(D,RO).main() @ &m: res]
-     + Pr[G2(D,RO).main() @ &m: res].
-  proof.
-    move=> Da1L Da2L.
-    cut ->: Pr[G2(D,RO).main() @ &m: res] = Pr[G1(D,RO).main() @ &m: mem G1.x ARO.qs].
-      byequiv (_: ={glob D} ==> res{1} = (mem G1.x ARO.qs){2})=> //.
-      proc.
-      call (_: ={glob ARO, glob RO}); first by sim.
-      rnd; call (_: ={glob ARO, glob RO}); first by sim.
-      by inline *; wp.
-    cut: Pr[G0(D,RO).main() @ &m: res] <= Pr[G1(D,RO).main() @ &m: res \/ mem G1.x ARO.qs].
-      byequiv (_: ={glob D} ==> !mem G1.x{2} ARO.qs{2} => ={res})=> //; last smt.
-      proc.
-      call (_: !mem G1.x{2} ARO.qs{2} =>
-               ={glob D, ARO.qs, x} /\
-               ARO.qs{2} = dom RO.m{2} /\
-               eq_except RO.m{1} RO.m{2} G1.x{2} ==>
-               !mem G1.x{2} ARO.qs{2} =>
-               ={ARO.qs, res} /\
-               ARO.qs{2} = dom RO.m{2} /\
-               eq_except RO.m{1} RO.m{2} G1.x{2}).
-        proc (mem G1.x ARO.qs)
-             (={ARO.qs} /\
-              ARO.qs{2} = dom RO.m{2} /\
-              eq_except RO.m{1} RO.m{2} G1.x{2})=> //;
-          first 2 smt.
-          proc; sp; if=> //; inline RO.o; auto; progress; first 5 last; last 7 smt.
-          case (x{2} = G1.x{2}); first smt.
-          by move=> neq; cut:= H0; rewrite eq_except_def; smt.
-          smt.
-          smt.
-          case (x{2} = G1.x{2}); first smt.
-          by move=> neq; cut:= H0; rewrite eq_except_def; smt.
-        by progress; proc; sp; if=> //; wp; call (lossless_o _); first smt.
-        by progress; proc; sp; if=> //; wp; call (lossless_o _); [smt | skip; smt].
-      inline RO.o; wp; rnd; wp.
-      call (_: ={glob ARO, glob RO} /\ ARO.qs{2} = dom RO.m{2}).
-        by proc; sp; if=> //; inline RO.o; auto; progress; smt.
-      by inline RO.init; auto; progress; expect 7 smt.
-    by rewrite Pr [mu_or]; smt.
-  qed.
-end ROM_Call.
-
 (* The type of plaintexts: bitstrings of length k *)
 type bits.
 op k: int.
@@ -226,15 +82,12 @@ module Hashed_ElGamal (H:Hash): Scheme = {
   }
 }.
 
-clone import ROM_Call as ROC with
+clone import ROM.ROM_BadCall as ROC with
   type from  <- group,
   type to    <- bits,
   op dsample <- fun (x:group), uniform,
   op qH      <- qH
 proof * by smt.
-
-import ROM.
-import Types.
 
 (* Adversary Definitions *)
 module type Adversary (O:ARO) = {
@@ -242,16 +95,9 @@ module type Adversary (O:ARO) = {
   proc guess(c:ciphertext): bool
 }.
 
-module Bounder'(A:Adversary,O:ARO) = {
-  module A' = A(ARO(O))
-
-  proc choose = A'.choose
-  proc guess  = A'.guess
-}.
-
 (* Specializing and merging the hash function *)
 module H:Hash = {
-  proc init(): unit = { RO.init(); ARO.qs = FSet.empty; }
+  proc init(): unit = { RO.init(); Log.qs = FSet.empty; }
   proc hash(x:group): bits = { var y; y = RO.o(x); return y; }
 }.
 
@@ -263,8 +109,8 @@ hoare Correctness: Correctness(S).main: true ==> res.
 proof. by proc; inline *; auto; progress; smt. qed.
 
 (* The reduction *)
-module SCDH_from_CPA(A:Adversary,O:ARO): SCDH.Adversary = {
-  module BA = Bounder'(A,O)
+module SCDH_from_CPA(A:Adversary,O:Oracle): SCDH.Adversary = {
+  module BA = A(Bound(O))
 
   proc solve(gx:group, gy:group): group set = {
     var m0, m1, h, b';
@@ -273,19 +119,19 @@ module SCDH_from_CPA(A:Adversary,O:ARO): SCDH.Adversary = {
     (m0,m1)  = BA.choose(gx);
     h        = $uniform;
     b'       = BA.guess(gy, h);
-    return ARO.qs;
+    return Log.qs;
   }
 }.
 
 (* We want to bound the probability of A winning CPA(Bounder(A,RO),S) in terms of
    the probability of B = CDH_from_CPA(SCDH_from_CPA(A,RO)) winning CDH(B) *)
 section.
-  declare module A: Adversary {RO, Bounder, ROC.G1, ROC.G2}.
+  declare module A: Adversary {RO, Log, OnBound.G1, OnBound.G2}.
 
   axiom chooseL (O <: ARO {A}): islossless O.o => islossless A(O).choose.
   axiom guessL (O <: ARO {A}) : islossless O.o => islossless A(O).guess.
 
-  local module BA = Bounder'(A,RO).
+  local module BA = A(Bound(RO)).
 
   local module G0 = {
     var gxy:group
@@ -313,10 +159,10 @@ section.
     proc.
     inline Hashed_ElGamal(H).kg Hashed_ElGamal(H).enc.
     swap{1} 8 -5.
-    call (_: ={glob H, ARO.qs}); first by sim.
+    call (_: ={glob H, Log.qs}); first by sim.
     wp; call (_: ={glob H}); first by sim.
     wp; rnd.
-    call (_: ={glob H, ARO.qs}); first by sim.
+    call (_: ={glob H, Log.qs}); first by sim.
     wp; do !rnd.
     by call (_: true ==> ={glob H}); first by sim.
   qed.
@@ -361,7 +207,7 @@ section.
       h       = $uniform;
       c       = (g ^ y, h ^^ (b ? m1 : m0));
       b'      = BA.guess(c);
-      return mem G2.gxy ARO.qs;
+      return mem G2.gxy Log.qs;
     }
   }.
 
@@ -393,38 +239,38 @@ section.
     }
   }.
 
-  local lemma G0_D &m: Pr[G0.main() @ &m: res] = Pr[ROC.G0(D,RO).main() @ &m: res].
+  local lemma G0_D &m: Pr[G0.main() @ &m: res] = Pr[OnBound.G0(D,RO).main() @ &m: res].
   proof.
     byequiv (_: ={glob A} ==> ={res})=> //.
     proc.
-    inline ROC.G0(D,RO).D.a1 ROC.G0(D,RO).D.a2; wp.
+    inline OnBound.G0(D,RO).D.a1 OnBound.G0(D,RO).D.a2; wp.
     conseq* (_: _ ==> ={b'} /\ b{1} = D.b{2})=> //.
-    by inline H.hash H.init; sim.
+    by inline H.hash; sim.
   qed.
 
-  local lemma G1_D &m: Pr[G1.main() @ &m: res] = Pr[ROC.G1(D,RO).main() @ &m: res].
+  local lemma G1_D &m: Pr[G1.main() @ &m: res] = Pr[OnBound.G1(D,RO).main() @ &m: res].
   proof.
     byequiv (_: ={glob A} ==> ={res})=> //.
     proc.
-    inline ROC.G1(D,RO).D.a1 ROC.G1(D,RO).D.a2; wp.
+    inline OnBound.G1(D,RO).D.a1 OnBound.G1(D,RO).D.a2; wp.
     conseq* (_: _ ==> ={b'} /\ b{1} = D.b{2})=> //.
-    by inline H.hash H.init; sim.
+    by inline H.hash; sim.
   qed.
 
-  local lemma G2_D &m: Pr[G2.main() @ &m: res] = Pr[ROC.G2(D,RO).main() @ &m: res].
+  local lemma G2_D &m: Pr[G2.main() @ &m: res] = Pr[OnBound.G2(D,RO).main() @ &m: res].
   proof.
     byequiv (_: ={glob A} ==> ={res})=> //.
     proc.
-    inline ROC.G2(D,RO).D.a1 ROC.G2(D,RO).D.a2; wp.
-    conseq* (_: _ ==> ={glob ARO, b'} /\ b{1} = D.b{2} /\ G2.gxy{1} = ROC.G2.x{2})=> //.
-    by inline H.hash H.init; sim.
+    inline OnBound.G2(D,RO).D.a1 OnBound.G2(D,RO).D.a2; wp.
+    conseq* (_: _ ==> ={glob Log, b'} /\ b{1} = D.b{2} /\ G2.gxy{1} = x{2})=> //.
+    by inline H.hash; sim.
   qed.
 
   local lemma G0_G1_G2 &m:
     Pr[G0.main() @ &m: res] <= Pr[G1.main() @ &m: res] + Pr[G2.main() @ &m: res].
   proof.
     rewrite (G0_D &m) (G1_D &m) (G2_D &m).
-    apply (Abstract_Bad D &m).
+    apply (OnBound.ROM_BadCall D _ _ &m).
       by progress; proc; auto; call (chooseL H _)=> //; auto; progress; smt. 
       by progress; proc; call (guessL H _)=> //; auto.
   qed.
@@ -452,26 +298,27 @@ section.
   proof.
     byequiv (_: ={glob A} ==> ={res})=> //.
     proc.
-    call (_: ={glob RO, glob ARO}); first by sim.
+    call (_: ={glob RO, glob Log}); first by sim.
     wp; rnd (fun h, h ^^ if b then m1 else m0){1}; rnd.
-    call (_: ={glob RO, glob ARO}); first by sim.
+    call (_: ={glob RO, glob Log}); first by sim.
     by inline H.init RO.init; auto; progress; smt.
   qed.
 
   local lemma Pr_G1' &m: Pr[G1'.main() @ &m: res] = 1%r/2%r.
   proof.
+    cut RO_o_ll:= RO_o_ll _; first smt.
     byphoare (_: true ==> res)=> //.
     proc.
     swap 7 3.
     rnd ((=) b').
     call (_: true);
       first by progress; apply (guessL O).
-      by proc; sp; if=> //; wp; call (lossless_o _); first smt.
+      by proc; sp; if=> //; wp; call (Log_o_ll RO _).
     auto.
     call (_: true);
       first by progress; apply (chooseL O).
-      by proc; sp; if=> //; wp; call (lossless_o _); first smt.
-    inline H.init RO.init; auto; progress; expect 3 smt.
+      by proc; sp; if=> //; wp; call (Log_o_ll RO _).
+    by inline H.init RO.init; auto; progress; expect 3 smt.
   qed.
 
   local module G2' = {
@@ -491,7 +338,7 @@ section.
       h        = $uniform;
       c        = (g ^ y, h);
       b'       = BA.guess(c);
-      return mem gxy ARO.qs;
+      return mem gxy Log.qs;
     }
   }.
 
@@ -499,14 +346,14 @@ section.
   proof.
     byequiv (_: ={glob A} ==> ={res})=> //.
     proc.
-    call (_: ={glob RO, glob ARO}); first by sim.
+    call (_: ={glob RO, glob Log}); first by sim.
     wp; rnd (fun h, h ^^ if b then m1 else m0){1}; rnd.
-    call (_: ={glob RO, glob ARO}); first by sim.
+    call (_: ={glob RO, glob Log}); first by sim.
     by inline H.init RO.init; auto; progress; smt.
   qed.
 
   local equiv G2'_SCDH: G2'.main ~ SCDH.SCDH(SCDH_from_CPA(A,RO)).main:
-    ={glob A} ==> res{1} = res{2} /\ card ARO.qs{1} <= qH.
+    ={glob A} ==> res{1} = res{2} /\ card Log.qs{1} <= qH.
   proof.
     proc.
     inline SCDH_from_CPA(A,RO).solve.
@@ -515,12 +362,12 @@ section.
     seq  8  7: (={glob BA} /\
                 c{1} = (gy, h){2} /\
                 G2'.gxy{1} = g ^ (x * y){2} /\
-                card ARO.qs{1} <= qH).
-      wp; rnd; call (_: ={glob H} /\ card ARO.qs{1} <= qH).
-        by proc; sp; if=> //; inline RO.o; auto; smt.
+                card Log.qs{1} <= qH).
+      wp; rnd; call (_: ={glob H} /\ card Log.qs{1} <= qH).
+        by proc; sp; if=> //; inline Bound(RO).LO.o RO.o; auto; smt.
       by inline H.init RO.init; auto; progress; smt.
-    call (_: ={glob H} /\ card ARO.qs{1} <= qH).
-      by proc; sp; if=> //; inline RO.o; auto; smt.
+    call (_: ={glob H} /\ card Log.qs{1} <= qH).
+      by proc; sp; if=> //; inline Bound(RO).LO.o RO.o; auto; smt.
     by skip; smt.
   qed.
       
@@ -544,8 +391,8 @@ section.
   by [].
 
   (** Composing reduction from CPA to SCDH with reduction from SCDH to CDH *)
-  lemma Security &m :
-      Pr[CPA(S,Bounder'(A,RO)).main() @ &m: res] - 1%r / 2%r <= 
+  lemma Security &m:
+      Pr[CPA(S,A(Bound(RO))).main() @ &m: res] - 1%r / 2%r <= 
       qH%r * Pr[CDH.CDH(SCDH.CDH_from_SCDH(SCDH_from_CPA(A,RO))).main() @ &m: res].
   proof.
     apply (Trans _ (Pr[SCDH.SCDH(SCDH_from_CPA(A,RO)).main() @ &m: res]));
