examples/prp_prf.ec
@@ -1,7 +1,7 @@
 require import Int.
 require import AWord.
 require import FSet.
-require import Map.
+require import FMap.
 require import Real.
 require import Distr.
 require import Sum.
@@ -31,24 +31,24 @@ op uniform : block distr = Block.Dword.dword.
 import Dexcepted.
 (* Abstract cipher *)
 module type AC = {
- fun f (x : block) : block
- fun init () : unit 
+ proc f (x : block) : block
+ proc init () : unit 
  }.
 
 module type AAC = {
- fun f (x : block) : block
+ proc f (x : block) : block
 }.
 
 module PRP : AC = {
  var m : (block, block) map
  var s : block set
  var bad : bool
- fun init() : unit ={
-  m = Map.empty;
+ proc init() : unit ={
+  m = FMap.empty;
   s = FSet.empty;
   bad = false;
  }
- fun f (x : block) : block ={
+ proc f (x : block) : block ={
   var y : block;
   if (!in_dom x m /\ card s < q) {
    y = $uniform;
@@ -59,37 +59,37 @@ module PRP : AC = {
    s = add y s;
    m.[x] = y;
   }
-  return proj (m.[x]);
+  return oget (m.[x]);
  }
 }.
 
 module PRF : AC = {
  var m : (block, block) map
  var s : block set
- fun init() : unit ={
-  m = Map.empty;
+ proc init() : unit ={
+  m = FMap.empty;
   s = FSet.empty;
  }
- fun f (x : block) : block = {
+ proc f (x : block) : block = {
   var y : block;
   if (!in_dom x m /\ card s < q) {
    y = $uniform;
    m.[x] = y;
    s = add y s; 
   }
-  return proj(m.[x]);
+  return oget (m.[x]);
  }
 }.
 
 module type Adv(M : AAC) =
 {
- fun a() : bool
+ proc a() : bool
 }.
 
 
 module M(C : AC, A_ : Adv) ={
  module A = A_(C)
- fun main() : bool = {
+ proc main() : bool = {
   var b : bool;
   C.init();
   b = A.a();
@@ -106,12 +106,12 @@ forall (M0 <: AAC), islossless M0.f => islossless A(M0).a.
 equiv eq1 : M(PRF,A).main ~ M(PRP,A).main : 
             ={glob A} ==> card (PRP.s{2}) <= q /\ (!PRP.bad{2} => ={res}).
 proof.
- fun.
+ proc.
  call (_ : PRP.bad,
            PRF.m{1} = PRP.m{2} /\ PRF.s{1} = PRP.s{2} /\ card (PRP.s{2}) <= q, 
            card (PRP.s{2}) <= q).
  by intros M0 Hmo; apply (losslessA M0) => //.
- fun.
+ proc.
  if;first by smt.
  seq 1 1: 
  ((! PRP.bad{2} /\ ={x,y} /\ PRF.m{1} = PRP.m{2}) /\ ! in_dom x{1} PRF.m{1} /\
@@ -121,19 +121,19 @@ proof.
  by wp;rnd{2};wp;skip;progress;smt.
  by wp;skip;progress;smt.
  by skip;smt.
- intros &m2 H;fun;if;wp.
- rnd Fun.cpTrue.
+ intros &m2 H;proc;if;wp.
+ rnd True.
  wp;skip;progress;by smt.
  skip;by smt.
- intros &m1;fun;if;wp.
+ intros &m1;proc;if;wp.
  seq 1: ((PRP.bad /\ true) /\ ! in_dom x PRP.m /\ card PRP.s < q);last by smt.
  trivial.
- rnd Fun.cpTrue; skip;by smt.
- if;[rnd Fun.cpTrue;wp|];skip;by smt.
+ rnd True; skip;by smt.
+ if;[rnd True;wp|];skip;by smt.
  by hoare;rnd;skip => //.
  by skip => //.
  inline PRF.init PRP.init;wp;skip;by smt.
-save.
+qed.
 
 lemma real_le_trans : forall(a b c : real),  
   a <= b => b <= c => a <= c by []. 
@@ -146,28 +146,54 @@ proof.
  intros => &m.
  apply (real_le_trans _ 
  Pr[ M(PRP,A).main() @ &m : (res || (PRP.bad /\  card PRP.s <= q))] _ _ _).
- equiv_deno(eq1) => // ;first by smt.
- rewrite Pr mu_or;by smt.
-save.
+ byequiv(eq1) => // ;first by smt.
+ rewrite Pr [mu_or];by smt.
+qed.
 
 (* assumed property *)
-axiom sum_prop :
-forall (n : int),
-0 <= n =>
-int_sum (lambda (x : int), x%r * (1%r / (2 ^ l)%r)) (intval 0 (n - 1)) <=
-n%r * (n - 1)%r * (1%r / (2 ^ l)%r).
-
+lemma sum_prop (n : int):
+  0 <= n =>
+  int_sum (fun x, x%r * (1%r / (2 ^ l)%r)) (intval 0 (n - 1))
+  <= n%r * (n - 1)%r * (1%r / (2 ^ l)%r).
+proof.
+  move=> leq0_n.
+  cut ->: int_sum (fun x, x%r * (1%r/(2^l)%r)) (intval 0 (n - 1))
+          = int_sum (fun x, x%r) (intval 0 (n - 1)) * (1%r/(2^l)%r).
+    rewrite /int_sum /intval.
+    move: leq0_n; elim/Induction.induction n.
+      cut ->: Interval.interval 0 (0 - 1) = FSet.empty by smt.
+      by rewrite !Monoid.Mrplus.sum_empty; smt.
+      move=> n leq0_n IH; cut ->: n + 1 - 1 = n by smt.
+      cut:= Monoid.Mrplus.sum_ij_le_r 0 n (fun x, x%r * (1%r/(2^l)%r)) _=> //.
+      rewrite /Monoid.Mrplus.sum_ij IH=> -> /=.
+      cut:= Monoid.Mrplus.sum_ij_le_r 0 n (fun x, x%r) _=> //.
+      rewrite /Monoid.Mrplus.sum_ij=> -> /=.
+      smt.
+  cut ->: int_sum (fun x, x%r) (intval 0 (n - 1)) = (n - 1)%r * n%r / 2%r.
+    rewrite /int_sum /intval.
+    move: leq0_n; elim/Induction.induction n.
+      cut ->: Interval.interval 0 (0 - 1) = FSet.empty by smt.
+      by rewrite !Monoid.Mrplus.sum_empty; smt.
+      move=> n leq0_n IH; cut ->: n + 1 - 1 = n by smt.
+      cut:= Monoid.Mrplus.sum_ij_le_r 0 n (fun x, x%r) _=> //.
+      by rewrite /Monoid.Mrplus.sum_ij IH=> -> /=; smt.
+  cut ->: (n - 1)%r * n%r / 2%r = n%r * (n - 1)%r * (1%r / 2%r) by smt.
+  cut ->: n%r * (n - 1)%r * (1%r / 2%r) * (1%r / (2^l)%r) = (n%r * (n - 1)%r * (1%r / (2^l)%r)) * 1%r / 2%r by smt.
+  cut ->: forall x, 0%r <= x => x * 1%r / 2%r <= x; first last; last 2 smt.
+  cut ->: n%r * (n - 1)%r = (n * (n - 1))%r by smt.
+  cut ->: forall x y, 0%r <= x => 0%r <= y => 0%r <= x * y; smt.  
+qed.
 
 lemma prob2 : forall &m, 
 Pr[ M(PRP,A).main() @ &m : PRP.bad /\ card PRP.s <= q] <= 
 q%r * (q-1)%r * (1%r / (2^l)%r).
 proof.
  intros => &m.
- fel 1 (card PRP.s) (lambda x, (x%r)* (1%r/(2^l)%r)) 
+ fel 1 (card PRP.s) (fun x, (x%r)* (1%r/(2^l)%r)) 
      q PRP.bad [PRP.f : (! in_dom x PRP.m /\ card PRP.s < q)] => //. 
   apply sum_prop;by smt.
   inline PRP.init;wp;skip;by smt.
-  fun;if;wp.
+  proc;if;wp.
   seq 1 : (mem y PRP.s) 
           ((card PRP.s)%r * (1%r / (2^l)%r)) (1%r) 
           (1%r - ((card PRP.s)%r * (1%r / (2^l)%r))) (0%r)
@@ -181,18 +207,18 @@ proof.
    (conseq (_ : _ : 0%r); last hoare=> //); intros=> _ _;
      (cut H: forall x y, 0%r <= x => 0%r < y => 0%r <= x * y; first smt);
      apply H; smt.
-   intros c;fun;if;last by skip;smt.
+   intros c;proc;if;last by skip;smt.
  
    wp;seq 1: ((! in_dom x PRP.m /\ card PRP.s < q) /\ c = card PRP.s /\
   ! in_dom x PRP.m /\ card PRP.s < q /\ in_supp y uniform); first by rnd.
    if;[rnd;wp|];skip;progress;by smt.
          
-  intros b c;fun;wp;if;last by skip;smt.
+  intros b c;proc;wp;if;last by skip;smt.
   seq 1:  ((! (! in_dom x PRP.m /\ card PRP.s < q) /\ PRP.bad = b /\ 
           card PRP.s = c) /\ ! in_dom x PRP.m /\ card PRP.s < q /\ 
           in_supp y uniform);first rnd;skip;by smt.
   if;[wp;rnd|];wp;skip;by smt.
-save.
+qed.
 
 
 lemma concl : forall &m, 
@@ -209,7 +235,7 @@ proof.
  by apply (prob2 &m).
  cut H1: forall (x y z : real), x <= y => z + x <= z + y;first by smt.
  by apply H1 => //.    
-save.
+qed.
 
 end section.
 
