theories/ROM.ec
@@ -41,16 +41,17 @@ theory Types.
 end Types.
 
 theory Lazy.
+  require import FSet.
+
   type from.
   type to.
 
   op dsample: from -> to distr.
 
-  clone import Types with
+  clone export Types with
     type from <- from,
     type to <- to,
     op dsample <- dsample.
-  require import FSet.
 
   module RO:Oracle = {
     var m:(from, to) map
@@ -67,30 +68,27 @@ theory Lazy.
     }
   }.
 
-  lemma lossless_init: islossless RO.init.
-  proof strict.
-  by proc; wp.
-  qed.
+  lemma RO_init_ll: islossless RO.init.
+  proof. by proc; wp. qed.
 
-  lemma lossless_o:
+  lemma RO_o_ll:
     (forall x, mu (dsample x) True = 1%r) =>
     islossless RO.o.
-  proof strict.
-  by intros=> dsampleL; proc; wp; rnd; skip; smt.
-  qed.
+  proof. by intros=> dsampleL; proc; auto; smt. qed.
 
-  equiv abstract_init:
-    RO.init ~ RO.init: true ==> ={glob RO}
-  by (proc; wp).
+  equiv RO_init_eq: RO.init ~ RO.init: true ==> ={glob RO}
+  by sim.
 
-  equiv abstract_o:
-    RO.o ~ RO.o: ={glob RO, x} ==> ={glob RO, res}
-  by (proc; sim).
+  equiv RO_o_eq: RO.o ~ RO.o: ={glob RO, x} ==> ={glob RO, res}
+  by sim.
+
+  hoare dom_RO_o d x': RO.o: x = x' /\ dom RO.m = d ==> dom RO.m = add x' d.
+  proof. by proc; auto; smt. qed.
 end Lazy.
 
 theory Eager.
   require import ISet.
-    import Finite.
+  (*---*) import Finite.
   require import FSet.
 
   type from.
@@ -98,7 +96,7 @@ theory Eager.
 
   op dsample: from -> to distr.
 
-  clone import Types with
+  clone export Types with
     type from <- from,
     type to <- to,
     op dsample <- dsample.
@@ -127,40 +125,36 @@ theory Eager.
     }
   }.
 
-  lemma lossless_init:
+  lemma RO_init_ll:
     finite univ<:from> =>
     (forall x, mu (dsample x) True = 1%r) =>
     islossless RO.init.
-  proof strict.
-  intros=> fType dsampleL; proc.
-  while (true) (card work).
-    by intros=> z; wp; rnd True; wp;
-       skip; smt.
-  by wp; skip; smt.
+  proof.
+    move=> fType dsampleL; proc.
+    while (true) (card work);
+    by auto; smt.
   qed.
 
-  lemma lossless_o: islossless RO.o.
-  proof strict.
-  by proc; wp.
-  qed.
+  lemma RO_o_ll: islossless RO.o.
+  proof. by proc; wp. qed.
 
-  lemma abstract_init:
+  lemma RO_init_eq:
     finite univ<:from> =>
-    equiv [RO.init ~ RO.init: true ==> ={glob RO} /\ forall x, in_dom x RO.m{1}].
-  proof strict.
-  intros=> fType; proc;
-  while (={glob RO, work} /\ forall x, !mem x work{1} => in_dom x RO.m{1}).
-    by wp; rnd; wp; skip; progress=> //; smt.
-  by wp; skip; smt.
-  qed.
+    equiv [RO.init ~ RO.init: true ==> ={glob RO}].
+  proof. by move=> fType; proc; while (={glob RO, work}); auto. qed.
 
-  equiv abstract_o: RO.o ~ RO.o: ={glob RO, x} ==> ={glob RO, res}
-  by (proc; wp).
+  equiv RO_o_eq: RO.o ~ RO.o: ={glob RO, x} ==> ={glob RO, res}
+  by sim.
+
+  lemma dom_RO_init x:
+    finite univ<:from> =>
+    hoare [RO.init: true ==> mem x (dom RO.m)].
+  proof. by move=> fType; proc; while (forall x, !mem x work => mem x (dom RO.m)); auto; smt. qed.
 end Eager.
 
 theory LazyEager.
   require import ISet.
-    import Finite.
+  (*---*) import Finite.
   require import FSet.
 
   type from.
@@ -168,265 +162,301 @@ theory LazyEager.
 
   op dsample: from -> to distr.
 
-  clone import Types with
+  clone Types with
     type from <- from,
     type to <- to,
     op dsample <- dsample.
 
-  clone import Lazy with
+  clone export Lazy with
     type from <- from,
     type to <- to,
     op dsample <- dsample.
 
-  clone import Eager with
+  clone export Eager with
     type from <- from,
     type to <- to,
     op dsample <- dsample.
 
   section.
-  declare module D:Dist {Lazy.RO,Eager.RO}.
+    declare module D:Dist {Lazy.RO,Eager.RO}.
 
-  local module IND_Lazy = {
-    module H:Oracle = {
-      var m:(from, to) map
+    local module IND_Lazy = {
+      module H:Oracle = {
+        var m:(from, to) map
 
-      proc init():unit = {
-        m = FMap.empty;
+        proc init():unit = {
+          m = FMap.empty;
+        }
+
+        proc o(x:from):to = {
+          var y:to;
+          y = $dsample x;
+          if (!in_dom x m) m.[x] = y;
+          return oget (m.[x]);
+        }
       }
-  
-      proc o(x:from):to = {
-        var y:to;
-        y = $dsample x;
-        if (!in_dom x m) m.[x] = y;
-        return oget (m.[x]);
+
+      proc resample(): unit = {
+        var work:from set;
+        var f:from;
+        var y,y0:to;
+
+        work = toFSet univ;
+        while (work <> FSet.empty)
+        {
+          f = pick work;
+          y = $dsample f;
+          if (!in_dom f H.m) H.m.[f] = y;
+          work = rm f work;
+        }
       }
-    }
 
-    proc resample(): unit = {
-      var work:from set;
-      var f:from;
-      var y,y0:to;
+      module D = D(H)
 
-      work = toFSet univ;
-      while (work <> FSet.empty)
-      {
-        f = pick work;
-        y = $dsample f;
-        if (!in_dom f H.m) H.m.[f] = y;
-        work = rm f work;
+      proc main(): bool = {
+        var b:bool;
+
+        H.init();
+        b = D.distinguish();
+        resample();
+
+        return b;
       }
-    }
+    }.
 
-    module D = D(H)
+    local lemma IND_Lazy:
+      finite univ<:from> =>
+      (forall x, mu (dsample x) True = 1%r) =>
+      equiv [IND(Lazy.RO,D).main ~ IND_Lazy.main: ={glob D} ==> ={res}].
+    proof.
+      move=> fromF dsampleL; proc; seq 2 2: (={b}).
+        call (_: Lazy.RO.m{1} = IND_Lazy.H.m{2}); first by sim.
+        by call (_: ={glob D} ==> Lazy.RO.m{1} = IND_Lazy.H.m{2});
+          first by proc; wp.
+      inline IND_Lazy.resample;
+      while{2} (true) (card work{2});
+        first by auto; smt.
+      by auto; smt.
+    qed.
 
-    proc main(): bool = {
-      var b:bool;
+    local module IND_Eager = {
+      module H = {
+        var m:(from,to) map
 
-      H.init();
-      b = D.distinguish();
-      resample();
-
-      return b;
-    }
-  }.
-
-  local lemma IND_Lazy:
-    finite univ<:from> =>
-    (forall x, mu (dsample x) True = 1%r) =>
-    equiv [IND(Lazy.RO,D).main ~ IND_Lazy.main: ={glob D} ==> ={res}].
-  proof strict.
-  intros=> fromF dsampleL; proc; seq 2 2: (={b}).
-    call (_: Lazy.RO.m{1} = IND_Lazy.H.m{2}); first by (proc; sim).
-    by call (_: ={glob D} ==> Lazy.RO.m{1} = IND_Lazy.H.m{2})=> //;
-      first by proc; wp.
-    inline IND_Lazy.resample;
-    while{2} (true) (card work{2}).
-      intros=> &m z; wp; rnd; wp; skip; progress=> //; last smt.
-      by rewrite card_rm_in ?mem_pick //; smt. (* This should definitely be a lemma in FSet. *)
-    by wp; skip; progress=> //; smt.
-  qed.
-
-  local module IND_Eager = {
-    module H = {
-      var m:(from,to) map
-
-      proc o(x:from): to = {
-        return oget (m.[x]);
+        proc o(x:from): to = {
+          return oget (m.[x]);
+        }
       }
-    }
 
-    proc resample(): unit = {
-      var work:from set;
-      var f:from;
-      var y,y0:to;
+      proc resample(): unit = {
+        var work:from set;
+        var f:from;
+        var y,y0:to;
 
-      work = toFSet univ;
-      while (work <> FSet.empty)
-      {
-        f = pick work;
-        y = $dsample f;
-        if (!in_dom f H.m) H.m.[f] = y;
-        work = rm f work;
+        work = toFSet univ;
+        while (work <> FSet.empty)
+        {
+          f = pick work;
+          y = $dsample f;
+          if (!in_dom f H.m) H.m.[f] = y;
+          work = rm f work;
+        }
       }
-    }
 
-    module D = D(H)
+      module D = D(H)
 
-    proc main(): bool = {
-      var b:bool;
+      proc main(): bool = {
+        var b:bool;
 
-      H.m = FMap.empty;
-      resample();
-      b = D.distinguish();
+        H.m = FMap.empty;
+        resample();
+        b = D.distinguish();
 
-      return b;
-    }
-  }.
+        return b;
+      }
+    }.
 
-  local lemma eager_query:
-    finite univ<:from> =>
-    (forall x, mu (dsample x) True = 1%r) =>
-    eager [IND_Eager.resample(); ,
-               IND_Eager.H.o ~ IND_Lazy.H.o,
-           IND_Lazy.resample();:
-      ={x} /\ IND_Eager.H.m{1} = IND_Lazy.H.m{2} ==>
-      ={res} /\ IND_Eager.H.m{1} = IND_Lazy.H.m{2}].
-  proof strict.
-  intros=> fromF dsampleL; eager proc.
-  inline IND_Eager.resample IND_Lazy.resample; swap{2} 4 -3.
-  seq 1 1: (={x,work} /\
-            IND_Eager.H.m{1} = IND_Lazy.H.m{2} /\
-            mem x{1} work{1});
-    first by wp; skip; smt.
-  case (!in_dom x{2} IND_Lazy.H.m{2}); [rcondt{2} 2; first by intros=> &m; rnd |
-                                        rcondf{2} 2; first by intros=> &m; rnd].
-    transitivity{1} {y0 = $dsample x;
-                     while (work <> FSet.empty) {
-                       f = pick work;
-                       y = $dsample f;
-                       if (!in_dom f IND_Eager.H.m)
-                         IND_Eager.H.m.[f] = if f = x then y0 else y;
-                       work = rm f work;
-                     }
-                     result = oget IND_Eager.H.m.[x]; }
-                     (={x,work,IND_Eager.H.m} ==> ={result,IND_Eager.H.m})
-                     ((={x,work} /\
-                      IND_Eager.H.m{1} = IND_Lazy.H.m{2} /\
-                      mem x{1} work{1}) /\
-                      !in_dom x{2} IND_Lazy.H.m{2} ==>
-                      ={result} /\ IND_Eager.H.m{1} = IND_Lazy.H.m{2}) => //.
-      by intros=> &1 &2 H; exists IND_Lazy.H.m{2}, x{2}, work{2}; generalize H.
-    transitivity{1} {while (work <> FSet.empty) {
-                       f = pick work;
-                       y = $dsample f;
-                       if (!in_dom f IND_Eager.H.m)
-                         IND_Eager.H.m.[f] = y;
-                       work = rm f work;
-                     }
-                     y0 = $dsample x;
-                     result = oget IND_Eager.H.m.[x]; }
-                     (={x,work,IND_Eager.H.m} ==> ={result,IND_Eager.H.m})
-                     (={x,work,IND_Eager.H.m} ==> ={result,IND_Eager.H.m})=> //.
-      by intros &1 &2 H; exists IND_Eager.H.m{2}, x{2}, work{2}; generalize H.
-    by sim; rnd{2}; sim true true: (={x,IND_Eager.H.m}); smt.
+    local lemma eager_query:
+      finite univ<:from> =>
+      (forall x, mu (dsample x) True = 1%r) =>
+      eager [IND_Eager.resample(); ,
+                 IND_Eager.H.o ~ IND_Lazy.H.o,
+             IND_Lazy.resample();:
+        ={x} /\ IND_Eager.H.m{1} = IND_Lazy.H.m{2} ==>
+        ={res} /\ IND_Eager.H.m{1} = IND_Lazy.H.m{2}].
+    proof.
+      move=> fromF dsampleL; eager proc.
+      inline IND_Eager.resample IND_Lazy.resample; swap{2} 4 -3.
+      seq 1 1: (={x,work} /\
+                IND_Eager.H.m{1} = IND_Lazy.H.m{2} /\
+                mem x{1} work{1});
+        first by auto; smt.
+      case (!in_dom x{2} IND_Lazy.H.m{2}); [rcondt{2} 2; first by auto |
+                                            rcondf{2} 2; first by auto].
+        transitivity{1} {y0 = $dsample x;
+                         while (work <> FSet.empty) {
+                           f = pick work;
+                           y = $dsample f;
+                           if (!in_dom f IND_Eager.H.m)
+                             IND_Eager.H.m.[f] = if f = x then y0 else y;
+                           work = rm f work;
+                         }
+                         result = oget IND_Eager.H.m.[x]; }
+                         (={x,work,IND_Eager.H.m} ==> ={result,IND_Eager.H.m})
+                         ((={x,work} /\
+                          IND_Eager.H.m{1} = IND_Lazy.H.m{2} /\
+                          mem x{1} work{1}) /\
+                          !in_dom x{2} IND_Lazy.H.m{2} ==>
+                          ={result} /\ IND_Eager.H.m{1} = IND_Lazy.H.m{2}) => //.
+          by move=> &1 &2 H; exists IND_Lazy.H.m{2}, x{2}, work{2}; generalize H.
+        transitivity{1} {while (work <> FSet.empty) {
+                           f = pick work;
+                           y = $dsample f;
+                           if (!in_dom f IND_Eager.H.m)
+                             IND_Eager.H.m.[f] = y;
+                           work = rm f work;
+                         }
+                         y0 = $dsample x;
+                         result = oget IND_Eager.H.m.[x]; }
+                         (={x,work,IND_Eager.H.m} ==> ={result,IND_Eager.H.m})
+                         (={x,work,IND_Eager.H.m} ==> ={result,IND_Eager.H.m})=> //.
+          by move=> &1 &2 H; exists IND_Eager.H.m{2}, x{2}, work{2}; generalize H.
+        by sim; rnd{2}; sim true true: (={x,IND_Eager.H.m}); smt.
 
-    wp; symmetry.
-    eager while (H:y0 = $dsample x; ~ y0 = $dsample x; : ={x} ==> ={y0})=> //; first by rnd.
-      swap{2} 5 -4; swap [2..3] -1; case ((x = pick work){1}).
-        by wp; rnd{2}; rnd; rnd{1}; wp; skip; smt.
-        by wp; do 2!rnd; wp; skip; smt.
+        wp; symmetry.
+        eager while (H:y0 = $dsample x; ~ y0 = $dsample x; : ={x} ==> ={y0})=> //; first by rnd.
+          swap{2} 5 -4; swap [2..3] -1; case ((x = pick work){1}).
+            by wp; rnd{2}; rnd; rnd{1}; wp; skip; smt.
+            by auto; smt.
+          by sim.
+
+        wp; while (={x, work} /\
+                   (!mem x work => in_dom x IND_Eager.H.m){1} /\
+                   IND_Lazy.H.m.[x]{2} = Some y0{1} /\
+                   if (in_dom x IND_Eager.H.m){1}
+                   then IND_Eager.H.m{1} = IND_Lazy.H.m{2}
+                   else eq_except IND_Eager.H.m{1} IND_Lazy.H.m{2} x{1}).
+          (* "expect 12 (move)" is used for catching changes in tactic behaviour early *)
+          auto; (progress; expect 12 move); last 2 first; first 11 smt.
+          case ((pick work = x){2})=> pick_x; last smt.
+          subst x{2}; generalize H8 H1; rewrite -neqF /eq_except=> -> /= eq_exc.
+          by apply map_ext=> x0; case (pick work{2} = x0); smt.
+        by auto; smt.
+
+      wp; while (={x,work} /\
+                 IND_Eager.H.m{1} = IND_Lazy.H.m{2} /\
+                 in_dom x{2} IND_Lazy.H.m{2} /\ 
+                 oget IND_Eager.H.m.[x]{1} = result{2}).
+         by auto; smt.
+      by auto; smt.
+    qed.
+
+    local lemma eager_aux:
+      finite univ<:from> =>
+      (forall x, mu (dsample x) True = 1%r) =>
+      equiv [IND_Lazy.main ~ IND_Eager.main: ={glob D} ==> ={res}].
+    proof.
+      move=> fromF dsampleL; proc; inline IND_Lazy.H.init.
+      seq 1 1: (={glob D} /\ IND_Lazy.H.m{1} = IND_Eager.H.m{2}); first by wp.
+      symmetry.
+      eager (H: IND_Eager.resample(); ~ IND_Lazy.resample();:
+                  IND_Eager.H.m{1} = IND_Lazy.H.m{2} ==> IND_Eager.H.m{1} = IND_Lazy.H.m{2}): 
+            (={glob D} /\ IND_Eager.H.m{1} = IND_Lazy.H.m{2})=> //;
+        first by sim.
+      eager proc H (IND_Eager.H.m{1} = IND_Lazy.H.m{2})=> //;
+        first by apply eager_query.
       by sim.
+    qed.
 
-    wp; while (={x, work} /\
-               (!mem x work => in_dom x IND_Eager.H.m){1} /\
-               IND_Lazy.H.m.[x]{2} = Some y0{1} /\
-               if (in_dom x IND_Eager.H.m){1}
-               then IND_Eager.H.m{1} = IND_Lazy.H.m{2}
-               else eq_except IND_Eager.H.m{1} IND_Lazy.H.m{2} x{1}).
-      (* We should have a good battery of lemmas on eq_except to deal with this *)
-      wp; rnd; wp; skip; progress.
-        smt.
-        smt.
-        smt.
-        by case ((pick work = x){2}); smt.
-        smt.
-        smt.
-        smt.
-        smt.
-        smt.
-        case ((pick work = x){2})=> pick_x; last smt.
-        subst x{2}; generalize H8 H1; rewrite -neqF eq_except_def=> -> /= eq_exc.
-        apply map_ext=> x0; case (pick work{2} = x0).
-          by intros=> <-; rewrite get_set_eq H0.
-          by intros=> neq_x0_pick; rewrite get_set_neq // eq_exc //.
-        by case ((pick work = x){2}); smt.
-        smt.
-    by wp; rnd; skip; progress=> //; smt.
+    local lemma IND_Eager:
+      finite univ<:from> =>
+      (forall x, mu (dsample x) True = 1%r) =>
+      equiv [IND_Eager.main ~ IND(Eager.RO,D).main: ={glob D} ==> ={res}].
+    proof.
+      move=> fromF dsampleL; proc.
+      call (_: (forall x, in_dom x IND_Eager.H.m{1}) /\ IND_Eager.H.m{1} = Eager.RO.m{2});
+        first by proc; skip; smt.
+      inline RO.init IND_Eager.resample.
+      while (={work} /\
+             (forall x, !in_dom x IND_Eager.H.m{1} <=>
+                        mem x work{1}) /\ IND_Eager.H.m{1} = Eager.RO.m{2}).
+        by auto; progress; smt.
+      by auto; smt.
+    qed.
 
-  wp; while (={x,work} /\
-             IND_Eager.H.m{1} = IND_Lazy.H.m{2} /\
-             in_dom x{2} IND_Lazy.H.m{2} /\ 
-             oget IND_Eager.H.m.[x]{1} = result{2}).
-     by wp; rnd; wp; skip; progress=> //; smt.
-  by wp; rnd{2}; skip; smt.
-  qed.
-
-  local lemma eager_aux:
-    finite univ<:from> =>
-    (forall x, mu (dsample x) True = 1%r) =>
-    equiv [IND_Lazy.main ~ IND_Eager.main: ={glob D} ==> ={res}].
-  proof strict.
-  intros=> fromF dsampleL; proc; inline IND_Lazy.H.init.
-  seq 1 1: (={glob D} /\ IND_Lazy.H.m{1} = IND_Eager.H.m{2}); first by wp.
-  symmetry;
-  eager (H: IND_Eager.resample(); ~ IND_Lazy.resample();:
-              IND_Eager.H.m{1} = IND_Lazy.H.m{2} ==> IND_Eager.H.m{1} = IND_Lazy.H.m{2}): 
-        (={glob D} /\ IND_Eager.H.m{1} = IND_Lazy.H.m{2})=> //;
-    first by sim.
-  eager proc H (IND_Eager.H.m{1} = IND_Lazy.H.m{2})=> //;
-    first by apply eager_query=> //.
-  by proc; sim.
-  qed.
-
-  local lemma IND_Eager:
-    finite univ<:from> =>
-    (forall x, mu (dsample x) True = 1%r) =>
-    equiv [IND_Eager.main ~ IND(Eager.RO,D).main: ={glob D} ==> ={res}].
-  proof strict.
-  intros=> fromF dsampleL; proc.
-  call (_: (forall x, in_dom x IND_Eager.H.m{1}) /\ IND_Eager.H.m{1} = Eager.RO.m{2}).
-    by proc; skip; smt.
-  inline RO.init IND_Eager.resample.
-    while (={work} /\ (forall x, !in_dom x IND_Eager.H.m{1} <=> mem x work{1}) /\ IND_Eager.H.m{1} = Eager.RO.m{2}).
-      by wp; rnd; wp; skip; progress=> //; smt.
-    by wp; skip; smt.
-  qed.
-
-  lemma eagerRO:
-    finite univ<:from> =>
-    (forall x, mu (dsample x) True = 1%r) =>
-    equiv [IND(Lazy.RO,D).main ~ IND(Eager.RO,D).main: ={glob D} ==> ={res}].
-  proof strict.
-  intros=> fromF dsampleL; bypr (res{1}) (res{2})=> //; intros=> &1 &2 a eq_D.
-  apply (eq_trans _ Pr[IND_Lazy.main() @ &1: a = res]);
-    first by byequiv (IND_Lazy _ _).
-  apply (eq_trans _ Pr[IND_Eager.main() @ &1: a = res]);
-    first by byequiv (eager_aux _ _).
-  by byequiv (IND_Eager _ _).
-  qed.
+    lemma eagerRO:
+      finite univ<:from> =>
+      (forall x, mu (dsample x) True = 1%r) =>
+      equiv [IND(Lazy.RO,D).main ~ IND(Eager.RO,D).main: ={glob D} ==> ={res}].
+    proof.
+      move=> fromF dsampleL; bypr (res{1}) (res{2})=> // &1 &2 a eq_D.
+      apply (eq_trans _ Pr[IND_Lazy.main() @ &1: a = res]);
+        first by byequiv (IND_Lazy _ _).
+      apply (eq_trans _ Pr[IND_Eager.main() @ &1: a = res]);
+        first by byequiv (eager_aux _ _).
+      by byequiv (IND_Eager _ _).
+    qed.
   end section.
 end LazyEager.
 
-theory Upto.
-  require import List.
+theory BoundedCall.
+  require import Int.
 
-  clone import Types.
-  clone import Lazy with
+  type from.
+  type to.
+
+  op dsample: from -> to distr.
+
+  op qH:int.
+
+  clone export Lazy with
     type from  <- from,
     type to    <- to,
     op dsample <- dsample.
 
-  module Queries (O:Oracle) = {
+  module Bound (O:Oracle) = {
+    var c:int
+
+    proc init(): unit = {
+      O.init();
+      c = 0;
+    }
+
+    proc o(x:from): to = {
+      var r = witness;
+
+      if (c < qH) {
+        r = O.o(x);
+        c = c + 1;
+      }
+      return r;
+    }
+  }.
+
+  lemma Bound_init_ll (O <: Oracle): islossless O.init => islossless Bound(O).init.
+  proof. by move=> O_init_ll; proc; wp; call O_init_ll. qed.
+
+  lemma Bound_o_ll (O <: Oracle): islossless O.o => islossless Bound(O).o.
+  proof. by move=> O_o_ll; proc; sp; if=> //; wp; call O_o_ll. qed.
+end BoundedCall.
+
+theory ListLog.
+  require import Int.
+  require import List.
+
+  type from.
+  type to.
+
+  op dsample: from -> to distr.
+
+  op qH:int.
+
+  clone export Lazy with
+    type from  <- from,
+    type to    <- to,
+    op dsample <- dsample.
+
+  module Log (O:Oracle) = {
     var qs:from list
 
     proc init(): unit = {
@@ -443,40 +473,445 @@ theory Upto.
     }
   }.
 
-  lemma Queries_initL (O <: Oracle):
-    islossless O.init =>
-    islossless Queries(O).init.
-  proof strict.
-  by intros=> O_initL; proc; wp; call O_initL.
-  qed.
+  lemma Log_init_ll (O <: Oracle): islossless O.init => islossless Log(O).init.
+  proof. by move=> O_init_ll; proc; wp; call O_init_ll. qed.
 
-  lemma Queries_oL (O <: Oracle):
-    islossless O.o =>
-    islossless Queries(O).o.
-  proof strict.
-  by intros=> O_oL; proc; call O_oL; wp.
-  qed.
+  lemma Log_o_ll (O <: Oracle): islossless O.o => islossless Log(O).o.
+  proof. by move=> O_oL; proc; call O_oL; wp. qed.
 
-  lemma Queries_o_stable (O <: Oracle) q:
-    islossless O.o =>
-    phoare[ Queries(O).o: mem q Queries.qs ==> mem q Queries.qs ] = 1%r.
-  proof strict.
-  by intros=> O_oL; proc; call O_oL; wp; skip;
-     progress; right.
-  qed.
+  lemma Log_o_stable (O <: Oracle) q:
+    islossless O.o => phoare[Log(O).o: mem q Log.qs ==> mem q Log.qs] = 1%r.
+  proof. by move=> O_o_ll; proc; call O_o_ll; auto; progress; right. qed.
 
-  equiv RO_upto_o r:
-    Queries(RO).o ~ Queries(RO).o:
-      !mem r Queries.qs{2} /\
-      ={x, Queries.qs} /\
-      eq_except RO.m{1} RO.m{2} r ==>
-      !mem r Queries.qs{2} =>
-      ={res, Queries.qs} /\
-      eq_except RO.m{1} RO.m{2} r.
-  proof strict.
-  by proc; inline RO.o; wp; rnd; wp; skip; progress; smt.
+  module Bound(O:Oracle) = {
+    module LO = Log(O)
+
+    proc init(): unit = {
+      Log(O).init();
+    }
+
+    proc o(x:from): to = {
+      var r = witness;
+
+      if (length Log.qs < qH) {
+        r = O.o(x);
+      }
+      return r;
+    }
+  }.
+end ListLog.
+
+theory SetLog.
+  require import Int.
+  require import FSet.
+
+  type from.
+  type to.
+
+  op dsample: from -> to distr.
+
+  op qH:int.
+
+  clone export Lazy with
+    type from  <- from,
+    type to    <- to,
+    op dsample <- dsample.
+
+  module Log(O:Oracle) = {
+    var qs:from set
+
+    proc init(): unit = {
+      O.init();
+      qs = FSet.empty;
+    }
+
+    proc o(x:from): to = {
+      var r;
+
+      r  = O.o(x);
+      qs = add x qs;
+      return r;
+    }
+  }.
+
+  lemma Log_init_ll (O <: Oracle): islossless O.init => islossless Log(O).init.
+  proof. by move=> O_init_ll; proc; wp; call O_init_ll. qed.
+
+  lemma Log_o_ll (O <: Oracle): islossless O.o => islossless Log(O).o.
+  proof. by move=> O_o_ll; proc; wp; call O_o_ll; wp. qed.
+
+  hoare Log_o_stable (O <: Oracle) x: Log(O).o: mem x Log.qs ==> mem x Log.qs.
+  proof. by proc; wp; call (_: true); skip; smt. qed.
+
+  module Bound(O:Oracle) = {
+    module LO = Log(O)
+
+    proc init = Log(O).init
+
+    proc o(x:from): to = {
+      var r = witness;
+
+      if (card Log.qs < qH) {
+        r = LO.o(x);
+      }
+      return r;
+    }
+  }.
+
+  lemma Bound_init_ll (O <: Oracle): islossless O.init => islossless Bound(O).init.
+  proof. by move=> O_init_ll; proc; wp; call O_init_ll. qed.
+
+  lemma Bound_o_ll (O <: Oracle): islossless O.o => islossless Bound(O).o.
+  proof. by move=> O_o_ll; proc; sp; if=> //; wp; call (Log_o_ll O _). qed.
+
+  hoare Bound_o_stable (O <: Oracle) x: Bound(O).o: mem x Log.qs ==> mem x Log.qs.
+  proof. by proc; sp; if=> //; wp; call (Log_o_stable O x). qed.
+
+  equiv Log_Bound (O <: Oracle {Log}) (D <: Dist {O,Log}):
+    IND(Bound(O),D).main ~ IND(Log(Bound(O)),D).main: ={glob O, glob D} ==> ={res}.
+  proof.
+    proc.
+    call (_: ={glob O} /\ card Log.qs{1} <= card Log.qs{2} /\ (card Log.qs{1} < qH => ={glob Log})).
+      proc*; inline Log(Bound(O)).o Bound(O).o Bound(O).LO.o.
+      sp; if; first smt.
+        by wp; call (_: true); auto; smt.
+        by auto; smt.
+    by inline *; wp; call (_: true).
   qed.
-end Upto.
+end SetLog.
+
+theory ROM_BadCall.
+  (** A generic argument allowing us to replace a single random
+      oracle query with freshly sampled randomness. We then bound
+      the probability of distinguishing the two modules by the
+      probability of a third module that simply returns whether
+      the replaced query has been guessed by the adversary.       *)
+  (** We want to be able to:
+        1) express the result on Log(O);
+        2) and use it on Bound(O)...
+      HOW? *)
+  require import Int.
+  require import Real.
+  require import FSet.
+
+  type from.
+  type to.
+
+  op dsample: from -> to distr.
+  axiom dsampleL x: mu (dsample x) True = 1%r.
+
+  op qH:int.
+
+  clone export SetLog with
+    type from  <- from,
+    type to    <- to,
+    op dsample <- dsample,
+    op qH      <- qH.
+
+  module type Dist(H:ARO) = {
+    proc a1(): from
+    proc a2(x:to): bool
+  }.
+
+  theory OnLog.
+    module G0(D:Dist, H:Oracle) = {
+      module D = D(Log(H))
+
+      proc main(): bool = {
+        var x, y, b;
+
+        Log(H).init();
+        x = D.a1();
+        y = H.o(x);
+        b = D.a2(y);
+        return b;
+      }
+    }.
+
+    module G1(D:Dist, H:Oracle) = {
+      module D = D(Log(H))
+
+      proc main(): bool = {
+        var x, y, b;
+
+        Log(H).init();
+        x = D.a1();
+        y = $dsample x;
+        b = D.a2(y);
+        return b;
+      }
+    }.
+
+    module G2(D:Dist, H:Oracle) = {
+      module D = D(Log(H))
+
+      proc main(): bool = {
+        var x, y, b;
+
+        Log(H).init();
+        x = D.a1();
+        y = $dsample x;
+        b = D.a2(y);
+        return mem x Log.qs;
+      }
+    }.
+
+    section.
+      declare module D : Dist {Log, RO}.
+      axiom Da1L (H <: Types.ARO {D}): islossless H.o => islossless D(H).a1.
+      axiom Da2L (H <: Types.ARO {D}): islossless H.o => islossless D(H).a2.
+
+      local module G1'(D:Dist, H:Oracle) = {
+        module D = D(Log(H))
+
+        var x:from
+
+        proc main(): bool = {
+          var y, b;
+
+          Log(H).init();
+          x = D.a1();
+          y = $dsample x;
+          b = D.a2(y);
+          return b;
+        }
+      }.
+
+      lemma ROM_BadCall &m:
+        Pr[G0(D,RO).main() @ &m: res] <= Pr[G1(D,RO).main() @ &m: res] + Pr[G2(D,RO).main() @ &m: res].
+      proof.
+        cut ->: Pr[G2(D,RO).main() @ &m: res] = Pr[G1'(D,RO).main() @ &m: mem G1'.x Log.qs].
+          byequiv (_: ={glob D} ==> res{1} = (mem G1'.x Log.qs){2})=> //.
+          proc.
+          call (_: ={glob Log, glob RO}); first by sim.
+          rnd; call (_: ={glob Log, glob RO}); first by sim.
+          by inline *; wp.
+        cut ->: Pr[G1(D,RO).main() @ &m: res] = Pr[G1'(D,RO).main() @ &m: res].
+          by byequiv (_: ={glob D} ==> ={res}); first by sim.
+        cut: Pr[G0(D,RO).main() @ &m: res] <= Pr[G1'(D,RO).main() @ &m: res \/ mem G1'.x Log.qs].
+          byequiv (_: ={glob D} ==> !mem G1'.x{2} Log.qs{2} => ={res})=> //; last smt.
+          proc.
+          call (_: mem G1'.x Log.qs,
+                   ={glob Log} /\
+                   Log.qs{2} = dom RO.m{2} /\
+                   eq_except RO.m{1} RO.m{2} G1'.x{2}).
+            by apply Da2L.
+            by proc; inline RO.o; auto; smt.
+            by progress; apply (Log_o_ll RO); apply (RO_o_ll _); smt.
+            progress; exists* G1'.x; elim* => x; conseq* (Log_o_ll RO _) (Log_o_stable RO x)=> //.
+            by apply (RO_o_ll _); smt.
+          inline RO.o; auto.
+          call (_: ={glob Log, glob RO} /\ Log.qs{2} = dom RO.m{2}).
+            by proc; inline RO.o; auto; smt.
+          by inline Log(RO).init RO.init; auto; smt.
+        by rewrite Pr [mu_or]; smt.
+      qed.
+    end section.
+  end OnLog.
+
+  theory OnBound.
+    module G0(D:Dist, H:Oracle) = {
+      module D = D(Bound(H))
+
+      proc main(): bool = {
+        var x, y, b;
+
+        Bound(H).init();
+        x = D.a1();
+        y = H.o(x);
+        b = D.a2(y);
+        return b;
+      }
+    }.
+
+    module G1(D:Dist, H:Oracle) = {
+      module D = D(Bound(H))
+
+      proc main(): bool = {
+        var x, y, b;
+
+        Bound(H).init();
+        x = D.a1();
+        y = $dsample x;
+        b = D.a2(y);
+        return b;
+      }
+    }.
+
+    module G2(D:Dist, H:Oracle) = {
+      module D = D(Bound(H))
+
+      proc main(): bool = {
+        var x, y, b;
+
+        Bound(H).init();
+        x = D.a1();
+        y = $dsample x;
+        b = D.a2(y);
+        return mem x Log.qs;
+      }
+    }.
+
+    section.
+      declare module D : Dist {Log, RO}.
+      axiom Da1L (H <: Types.ARO {D}): islossless H.o => islossless D(H).a1.
+      axiom Da2L (H <: Types.ARO {D}): islossless H.o => islossless D(H).a2.
+
+      local module G1'(D:Dist, H:Oracle) = {
+        module D = D(Bound(H))
+
+        var x:from
+
+        proc main(): bool = {
+          var y, b;
+
+          Log(H).init();
+          x = D.a1();
+          y = $dsample x;
+          b = D.a2(y);
+          return b;
+        }
+      }.
+
+      lemma ROM_BadCall &m:
+        Pr[G0(D,RO).main() @ &m: res] <= Pr[G1(D,RO).main() @ &m: res] + Pr[G2(D,RO).main() @ &m: res].
+      proof.
+        cut ->: Pr[G2(D,RO).main() @ &m: res] = Pr[G1'(D,RO).main() @ &m: mem G1'.x Log.qs].
+          byequiv (_: ={glob D} ==> res{1} = (mem G1'.x Log.qs){2})=> //.
+          proc.
+          call (_: ={glob Log, glob RO}); first by sim.
+          rnd; call (_: ={glob Log, glob RO}); first by sim.
+          by inline *; wp.
+        cut ->: Pr[G1(D,RO).main() @ &m: res] = Pr[G1'(D,RO).main() @ &m: res].
+          by byequiv (_: ={glob D} ==> ={res}); first by sim.
+        cut: Pr[G0(D,RO).main() @ &m: res] <= Pr[G1'(D,RO).main() @ &m: res \/ mem G1'.x Log.qs].
+          byequiv (_: ={glob D} ==> !mem G1'.x{2} Log.qs{2} => ={res})=> //; last smt.
+          proc.
+          call (_: mem G1'.x Log.qs,
+                   ={glob Log} /\
+                   Log.qs{2} = dom RO.m{2} /\
+                   eq_except RO.m{1} RO.m{2} G1'.x{2}).
+            by apply Da2L.
+            by proc; inline Bound(RO).LO.o RO.o; sp; if=> //; auto; smt.
+            by progress; apply (Bound_o_ll RO); apply (RO_o_ll _); smt.
+            progress; exists* G1'.x; elim* => x; conseq* (Bound_o_ll RO _) (Bound_o_stable RO x)=> //.
+            by apply (RO_o_ll _); smt.
+          inline RO.o; auto.
+          call (_: ={glob Log, glob RO} /\ Log.qs{2} = dom RO.m{2}).
+            by proc; inline Bound(RO).LO.o RO.o; sp; if=> //; auto; smt.
+          by inline Bound(RO).init Log(RO).init RO.init; auto; smt.
+        by rewrite Pr [mu_or]; smt.
+      qed.
+    end section.
+  end OnBound.    
+end ROM_BadCall.
+
+theory ROM_Bad.
+  (** This theory (and its final result FEL_ROM) abstracts away from the
+      Failure Event Lemma for Random Oracles, allowing it to be used at
+      a high-level of abstraction, without worrying about fel internals. *)
+  require import Int.
+  require import Real.
+  require import Sum. (* for the FEL tactic *)
+
+  type from.
+  type to.
+
+  op dsample: from -> to distr.
+  axiom dsampleL x: mu (dsample x) True = 1%r.
+
+  op qH:int.
+  axiom qH_pos: 0 < qH.
+
+  clone export BoundedCall with
+    type from  <- from,
+    type to    <- to,
+    op dsample <- dsample,
+    op qH      <- qH.
+
+  module type Dist(H:Oracle) = {
+    proc distinguish(): bool {H.o}
+  }.
+
+  module Experiment(H:Oracle,D:Dist) = {
+    module D = D(Bound(H))
+
+    proc main(): bool = {
+      var b;
+
+      Bound(H).init();
+      b = D.distinguish();
+      return b;
+    }
+  }.
+
+  section.
+    (** Note that the proof does not depend at all on the fact that O1 and O2
+        are random oracles. This argument could (and should) be generalized to
+        any two oracles whose probability of behaving differently on a single
+        query is bounded. *)
+    declare module O1 : Oracle {Bound}.
+    axiom O1_o_ll: islossless O1.o.
+
+    declare module O2 : Oracle {O1,Bound}.
+    axiom O2_o_ll: islossless O2.o.
+
+    declare module D : Dist {O1,O2,Bound}.
+    axiom D_distinguish_ll (O <: Oracle {D}): islossless O.o => islossless D(O).distinguish.
+
+    lemma FEL_ROM (bad: (glob O2) -> bool)
+                  (Phi: (glob O1) -> (glob O2) -> bool) eps &m:
+      0%r <= eps => (* should be derivable from phoare but isn't *)
+      hoare [O2.init: true ==> !bad (glob O2)] =>
+      equiv [O1.init ~ O2.init: true ==> Phi (glob O1){1} (glob O2){2}] =>
+      hoare [O2.o: bad (glob O2) ==> bad (glob O2)] =>
+      phoare [O2.o: !bad (glob O2) ==> bad (glob O2)] <= eps =>
+      equiv [O1.o ~ O2.o: !bad (glob O2){2} /\ ={x} /\ Phi (glob O1){1} (glob O2){2} ==>
+                          !bad (glob O2){2} => ={res} /\ Phi (glob O1){1} (glob O2){2}] =>
+      Pr[Experiment(O1,D).main() @ &m: res] <= Pr[Experiment(O2,D).main() @ &m: res] + qH%r * eps.
+    proof.
+      move=> eps_pos badinit eq_init bad_preserved bad1 eq_upto.
+      apply (Trans _ (Pr[Experiment(O2,D).main() @ &m: res] + Pr[Experiment(O2,D).main() @ &m: bad (glob O2)])).
+        cut: Pr[Experiment(O1,D).main() @ &m: res] <= Pr[Experiment(O2,D).main() @ &m: res \/ bad (glob O2)].
+          byequiv (_: ={glob D} ==> !bad (glob O2){2} => ={res})=> //; last smt.
+          proc.
+          call (_: bad (glob O2),
+                   ={glob Bound} /\
+                   Phi (glob O1){1} (glob O2){2}).
+            by apply D_distinguish_ll.
+            by proc; sp; if=> //; wp; call eq_upto.
+            by progress; proc; sp; if=> //; wp; call O1_o_ll.
+            by progress; proc; sp; if=> //; wp;
+               call (_: bad (glob O2) ==> bad (glob O2));
+                 first by conseq* O2_o_ll bad_preserved.
+          call (_: true ==> ={glob Bound} /\ Phi (glob O1){1} (glob O2){2} /\ !bad (glob O2){2}).
+            proc; inline Bound(O1).init Bound(O2).init; wp.
+            by call (_: true ==> Phi (glob O1){1} (glob O2){2} /\ !bad (glob O2){2});
+                 first conseq* eq_init _ badinit=> //.
+          by skip; smt.
+        by rewrite Pr [mu_or]; smt.
+      cut: Pr[Experiment(O2,D).main() @ &m: bad (glob O2)] <= qH%r * eps.
+        cut ->: Pr[Experiment(O2,D).main() @ &m: bad (glob O2)]
+                = Pr[Experiment(O2,D).main() @ &m: bad (glob O2) /\ Bound.c <= qH].
+          byequiv (_: ={glob D, glob O2} ==> bad (glob O2){1} <=> bad (glob O2){2} /\ Bound.c{2} <= qH)=> //.
+          proc.
+          call (_: ={glob O2, glob Bound} /\ Bound.c{2} <= qH)=> //.
+            by proc; sp; if=> //; wp; call (_: true); skip; smt.
+          call (_: ={glob O2} ==> ={glob O2, glob Bound} /\ Bound.c{2} <= qH).
+            by proc*; inline Bound(O2).init; wp; call (_: true); skip; smt.
+          done.
+        fel 1 Bound.c (fun x, eps) qH (bad (glob O2)) [Bound(O2).o: (Bound.c < qH)]=> //.
+          smt.
+          by call (_: true ==> !bad (glob O2) /\ Bound.c = 0);
+            first proc; wp; call badinit.
+          proc; sp; if=> //; last by hoare.
+          by wp; call (_: !bad (glob O2) ==> bad (glob O2)).
+          by progress; proc; sp; if=> //; wp; call (_: true); skip; smt.
+          by progress; proc; rcondf 2; auto; smt.
+      smt.
+    qed.
+  end section.
+end ROM_Bad.
 
 (*
 theory Wrappers.
